Notes upload

CoqExamples/expr_to_stack_machine.v
@@ -21,18 +21,22 @@ Fixpoint compile (e : exp) : program :=
     | Const n => [Push n]
     | Binop e1 o e2 => let p1 := compile e1 in 
                         let p2 := compile e2 in 
-                        p1 ++ p2 ++ [Exe o]
+                        p2 ++ p1 ++ [Exe o]
   end.
 
-(* When you don't want to really make it a definition *)
+(* When you don't want to really make it a definition use Example *)
 Example e1 := Binop (Const 2) Plus (Const 3).
 Example e2 := Binop e1 Minus (Const 5).
 
 Compute compile e2.
+(* There is a bug in the compiler - the order of operations is not correct *)
 
 Locate "+".
 Check Nat.add.
 Search (nat -> nat -> nat).
+
+
+(* Denotational Semantics: The meaning of stuff *)
 
 Definition opDenote (o : op) : nat -> nat -> nat :=
   match o with 
@@ -51,7 +55,7 @@ Definition stack := list nat.
 Definition instDenote (i : inst) (st : stack) : option stack :=
   match (i, st) with
   | (Push n, _) => Some (n::st)
-  | (Exe o, x::y::rest) => Some (opDenote o x y :: rest)
+  | (Exe o, x::y::rest) => Some ((opDenote o x y) :: rest)
   | _ => None
   end.
 
@@ -77,3 +81,36 @@ Definition sfun (ostp : option stack) (i : inst) :=
 
 Definition pDenote (p : program) (st : stack) : option stack :=
   List.fold_left sfun p (Some st).
+
+Theorem correct (e : exp): forall (st : stack), pDenote (compile e) st = Some (expDenote e :: st).
+  induction e.
+  - intros st. compute; trivial.
+  - intros st. simpl.
+Abort.
+(* Can't prove because it's a weak lemma and hence has weak induction hypothesis *)
+
+Theorem gen_correct (e : exp): forall (pg : program) (st : stack), pDenote (compile e ++ pg) st = pDenote pg (expDenote e :: st).
+  induction e.
+  - intros pg st; unfold pDenote; simpl; trivial.
+  - intros pg st; simpl.
+    Search ((_ ++ (_ ++ _) = _)).
+    rewrite <- app_assoc.
+    rewrite IHe2.
+    rewrite <- app_assoc.
+    rewrite IHe1.
+    unfold pDenote.
+    simpl.
+    unfold instDenote.
+    trivial.
+Qed.
+
+Theorem correct' (e : exp): forall (st : stack), pDenote (compile e) st = Some (expDenote e :: st).
+  intro st.
+(* We want to rewrite compile e as compile e ++ [] *)
+  Search ( _ ++ [] = _).
+  (* to rewrite  *)
+  Check app_nil_r.
+  rewrite <- (app_nil_r (compile e)).
+  rewrite gen_correct.
+  unfold pDenote; simpl; trivial.
+Qed.
