CoqExamples/bool_nat_expr.v
@@ -1,0 +1,30 @@
+Variant sort: Type := NAT | BOOL.
+Inductive exp: sort -> Type :=
+| Bconst: bool -> exp BOOL
+| Nconst: nat -> exp NAT
+| Plus: exp NAT -> exp NAT -> exp NAT
+| And: exp BOOL -> exp BOOL -> exp BOOL
+| If{s}: exp BOOL -> exp s -> exp s -> exp s.
+
+Definition sortDenote (s: sort): Set :=
+  match s with
+  | NAT => nat
+  | BOOL => bool
+  end.
+
+Search (bool -> bool -> bool).
+
+Fixpoint expDenote {s} (e: exp s): sortDenote s :=
+  match e with
+    (* In older versions of coq you would have to write an explicit match which newer versions of coq manages to infer and rewrite:
+       match e in exp s0 as e0 return sortDenote s0 with
+    *)
+  | Bconst b => b
+  | Nconst n => n
+  | Plus e1 e2 => (expDenote e1) + (expDenote e2)
+  | And e1 e2 => andb (expDenote e1) (expDenote e2)
+  | If e1 e2 e3 => if (expDenote e1) then (expDenote e2) else (expDenote e3)
+  end.
+
+Check expDenote.
+Print expDenote.
