CoqExamples/test1.v
@@ -1,3 +1,4 @@
+(* 2023 Test 1 *)
 (* Question 2*)
 Definition myand (P Q : bool) : bool :=
   match Q with
@@ -42,7 +43,7 @@ Definition mult (x y : nat) : nat := match y with
   | S y_minus1 => plus x (mult x y_minus1)
 end.
 
-(* Question 5*)
+(* Question 5 - Even Proposition*)
 Check Prop.
 Inductive Even : nat -> Prop :=
 | Even_O : Even O
@@ -58,3 +59,56 @@ Check True.
 Inductive Odd : nat -> Prop :=
 | Odd_1 : Odd (S O)
 | Odd_SS : forall n, Odd n -> Odd (S (S n)).
+
+(* Question 5 - Prisoners and Guards *)
+Print bool.
+Inductive Prisoner: Set := prisoner.
+Inductive Guard: Set := guard.
+Check Prisoner.
+Print Prisoner.
+
+Inductive valid_line_of_prisoners_and_guards := EmptyLine
+  | LonePrisoner: Prisoner -> valid_line_of_prisoners_and_guards
+  | ConsGuard: Guard -> valid_line_of_prisoners_and_guards -> valid_line_of_prisoners_and_guards
+  | ConsPrisonerWithGuard: Prisoner -> Guard -> valid_line_of_prisoners_and_guards -> valid_line_of_prisoners_and_guards.
+Check valid_line_of_prisoners_and_guards.
+Print valid_line_of_prisoners_and_guards.
+
+(* 14 Feb 2025 Test 1 *)
+(* Question 1 *)
+Inductive expr := Const (n : nat) | Plus (e1 e2 : expr) | Minus (e1 e2 : expr).
+
+Fixpoint countOp (e : expr) : nat :=
+  match e with 
+  | Const _ => 0
+  | Plus e1 e2 => countOp e1 + countOp e2 + 1
+  | Minus e1 e2 => countOp e1 + countOp e2 + 1
+  end.
+
+(* Question 3 *)
+Fixpoint plus' (a b : nat) : nat :=
+  match a with
+  | O => b
+  | S a_minus1 => S (plus' a_minus1 b)
+  end.
+
+Fixpoint mult' (a b : nat) : nat :=
+  match a with
+  | O => O
+  | S a_minus1 => plus' b (mult' a_minus1 b)
+  end.
+
+(* Question 4 *)
+Lemma implies : forall P Q : Prop, (not P \/ Q) -> (P -> Q).
+Proof.
+  refine (fun P Q nPorQ => match nPorQ with
+                           | or_introl nP => fun p: P => 
+                               let absurd (f : False) : Q := match f with end
+                           in absurd (nP p)
+                           | or_intror q => fun _ => q
+                           end).
+Qed.
+
+(* Lemma implies' : forall P Q : Prop, (P -> Q) -> (not P \/ Q). *)
+(* Proof. *)
+(*   refine (fun P Q PtoQ => _). *)
