CoqExamples/absurd_foo.v
@@ -1,0 +1,11 @@
+Definition foo (n : nat) : match n with
+                            | 0 => bool
+                            | S _ => nat 
+                            end 
+  := match n with
+      | 0 => true
+      | S _ => 42
+      end.
+
+Check foo.
+Print foo.
