CoqExamples/list.v
@@ -1,0 +1,4 @@
+Check list.
+Print list.
+Check nil.
+Check cons.
