CoqExamples/recover.v
@@ -1,0 +1,16 @@
+Check option.
+Print option.
+
+Definition recover {A} (o : option A) : match o with
+                                            | Some _ => A
+                                            | None => unit
+                                          end :=
+  match o with
+    | Some a => a
+    | None => tt
+  end.
+
+Check recover.
+Print recover.
+
+(* Definition something: nat = recover (hd ... ). *)
